add benchmarks + fix build
benchmarks seem ok for deletion too
- way faster
- correct complexity O(log n)

test.c
@@ -19,11 +19,20 @@ int main(int argc, char** argv) {
   //uint64_t r = P1_UInt32_main4 ();
   //printf("r=%lui\n", r);
   uint64_t x = strtoull(argv[1], NULL, 0);
-  uint64_t s = 0;
-  void* ptr = P1_UInt32_main5(x);
-  s = P1_UInt32_sot_wds(ptr);
-  printf("s=%lui\n", s);
-  uint64_t r = P1_UInt32_main6_aux(ptr, x);
-  printf("r=%lui\n", r);
+  uint64_t s1 = 0;
+  uint64_t s2 = 0;
+  uint64_t r1 = 0;
+  uint64_t r2 = 0;
+  void* ptr = NULL;
+  ptr = P1_UInt32_main5(x);
+  s1 = P1_UInt32_sot_wds(ptr);
+  printf("s1=%lui\n", s1);
+  r1 = P1_UInt32_main6_aux(ptr, x, true);
+  printf("r1=%lui\n", r1);
+  ptr = P1_UInt32_main7_aux (ptr, x);
+  s2 = P1_UInt32_sot_wds(ptr);
+  printf("s2=%lui\n", s2);
+  r2 = P1_UInt32_main6_aux(ptr, x, false);
+  printf("r2=%lui\n", r2);
   return 0;
 }
